## 4 Completar las pre o post-conditiones faltantes con predicados que hagan a cada tripla de Hoare valida:

### a) $\{x = y\}\ \  x := y ∗ 2\ \  Q$

$$
    Q \equiv \{x = 2 * y\}
$$

### b) $P\ \  x := x + 3\ \  \{x = z\}$

$$
    P \equiv wp(x := x + 3, \{x = z\})
                = \{x = z - 3\}
$$

### c) $P\ \  x := x + 1;\ y := y ∗ x\ \  \{y = 2 ∗z\}$

$$
\begin{split}
    P   &\equiv wp(x := x + 1, wp(y := y ∗ x, \{y = 2 ∗ z\}))\\
        &=      wp(x := x + 1, \{y * x = 2 ∗ z\})\\
        &=      \{y * (x + 1) = 2 ∗ z\}
\end{split}
$$


### d) $P\ \  if\ x > 0\ then\ y := x\ else\ y := 0\ fi\ \  \{y > 0\}$

$$
\begin{split}
    P   &\equiv wp(if\ x > 0\ then\ y := x\ else\ y := 0\ fi\, \{y > 0\})\\
        &=      (x > 0 \wedge wp(y := x, \{y > 0\})) \vee (x \leq 0 \wedge wp(y := 0, \{y > 0\}))\\
        &=     (x > 0 \wedge \{x > 0\}) \vee  (x \leq 0 \wedge \{0 > 0\})\\
        &=     \{x > 0\}\\
\end{split}
$$
